io/case-studies/webserver/StlcHandlers.fst
@@ -30,35 +30,35 @@ let handler_env =
   (extend TBytes empty))))) (* req *)
 
 let bt_handler (e:exp) (h:typing handler_env e (TSum TUnit TExn)) : tgt_handler =
- fun #fl sec_io (client : int) (req : Bytes.bytes) (send : Bytes.bytes -> MIOpi (either unit exn) fl pi _) ->
+ fun #fl sec_io (client : int) (req : Bytes.bytes) (send : Bytes.bytes -> MIOpi (either unit exn) fl sgm _) ->
    let client : FStar.Universe.raise_t file_descr = FStar.Universe.raise_val client in
-   let write : FStar.Universe.raise_t file_descr * FStar.Universe.raise_t bytes -> MIOpi (either (FStar.Universe.raise_t unit) (FStar.Universe.raise_t exn)) fl pi _ = fun fdb ->
+   let write : FStar.Universe.raise_t file_descr * FStar.Universe.raise_t bytes -> MIOpi (either (FStar.Universe.raise_t unit) (FStar.Universe.raise_t exn)) fl sgm _ = fun fdb ->
      let fd = FStar.Universe.downgrade_val (fst fdb) in
      let b = FStar.Universe.downgrade_val (snd fdb) in
      match sec_io Write (fd, b) with
      | Inl unit -> Inl (FStar.Universe.raise_val unit)
      | Inr ex -> Inr (FStar.Universe.raise_val ex) in
-   let socket : FStar.Universe.raise_t unit -> MIOpi (either (FStar.Universe.raise_t file_descr) (FStar.Universe.raise_t exn)) fl pi _ = fun _u ->
+   let socket : FStar.Universe.raise_t unit -> MIOpi (either (FStar.Universe.raise_t file_descr) (FStar.Universe.raise_t exn)) fl sgm _ = fun _u ->
      match sec_io Socket () with
      | Inl fd -> Inl (FStar.Universe.raise_val fd)
      | Inr ex -> Inr (FStar.Universe.raise_val ex) in
-   let openfile : FStar.Universe.raise_t string -> MIOpi (either (FStar.Universe.raise_t file_descr) (FStar.Universe.raise_t exn)) fl pi _ = fun s ->
+   let openfile : FStar.Universe.raise_t string -> MIOpi (either (FStar.Universe.raise_t file_descr) (FStar.Universe.raise_t exn)) fl sgm _ = fun s ->
      let s = FStar.Universe.downgrade_val s in
      match sec_io Openfile (s, [O_RDWR], 0x650) with
      | Inl fd -> Inl (FStar.Universe.raise_val fd)
      | Inr ex -> Inr (FStar.Universe.raise_val ex) in
-   let send : FStar.Universe.raise_t bytes -> MIOpi (either (FStar.Universe.raise_t unit) (FStar.Universe.raise_t exn)) fl pi _ = fun b -> match send (FStar.Universe.downgrade_val b) with
+   let send : FStar.Universe.raise_t bytes -> MIOpi (either (FStar.Universe.raise_t unit) (FStar.Universe.raise_t exn)) fl sgm _ = fun b -> match send (FStar.Universe.downgrade_val b) with
      | Inl unit -> Inl (FStar.Universe.raise_val unit)
      | Inr ex -> Inr (FStar.Universe.raise_val ex) in
    let req : FStar.Universe.raise_t bytes = FStar.Universe.raise_val req in
    let handler_venv = 
-     vextend #fl #mymst #pi #_ openfile (
-     vextend #fl #mymst #pi #_ socket (
-     vextend #fl #mymst #pi #(TArr (TPair TFDesc TBytes) (TSum TUnit TExn)) write (
-     vextend #fl #mymst #pi #TFDesc client (
-     vextend #fl #mymst #pi #(TArr TBytes (TSum TUnit TExn)) send (
-     vextend #fl #mymst #pi #TBytes req (
-     vempty #fl #pi #mymst)))))) in
+     vextend #fl #mymst #sgm #_ openfile (
+     vextend #fl #mymst #sgm #_ socket (
+     vextend #fl #mymst #sgm #(TArr (TPair TFDesc TBytes) (TSum TUnit TExn)) write (
+     vextend #fl #mymst #sgm #TFDesc client (
+     vextend #fl #mymst #sgm #(TArr TBytes (TSum TUnit TExn)) send (
+     vextend #fl #mymst #sgm #TBytes req (
+     vempty #fl #sgm #mymst)))))) in
    let v = exp_to_fstar handler_env e (TSum TUnit TExn) h handler_venv in
    match v with
    | Inl v -> Inl (FStar.Universe.downgrade_val v)
