io/MIO.Sig.Call.fst
@@ -7,5 +7,5 @@ assume val print_string2 : string -> Tot bool
 (** This file is replaced during linking with a file that contains the real
 implementation of the commands. **)
 
-let mio_call (#mst:mst) caller (cmd:cmds) (arg:(mio_sig mst).args cmd) : mio mst ((mio_sig mst).res cmd arg) =
+let mio_call (#mst:mstate) caller (cmd:cmds) (arg:(mio_sig mst).args cmd) : mio mst ((mio_sig mst).res cmd arg) =
   Call caller cmd arg Return
